Give, with derivations, the principle types for the terms $\lambda x y z . x z (y z)$, $\lambda x y . x$, $\lambda x y . x y$ and $\lambda x . x$ in Curry's system.
$$\begin{align*}
    PPc\ \lambda x . x &= \left< \Pi, P \right>\ \text{where} \\
    x \in (x) \implies \left< \Pi', P' \right> &= PPc\ x = \left< x : A, A \right> \\
    x \in (x) \implies \Pi &= \Pi'\\
    \\
    \text{finally,}\ \left< \Pi, P \right> &= \left< \Pi', A \to A \right> 
\end{align*}$$
==Not as above, see **below**.==

```
              7
          ---------
           3    6
          --- -----
λ x y z . x z (y z)
          | |  | |
          1 2  4 5

4 |-> 5 -> 6
3 |-> 6 -> 7
2 |-> 5

Therefore:

(1 |-> 2 -> 3) |-> 2 -> 6 -> 7

x : 5 |-> 6 |-> 7
y : 5 |-> 6
z : 5

Finally:

(5 -> 6 -> 7) -> (5 -> 6) -> 5 -> 7
(A -> B -> C) -> (A -> B) -> A -> C
```

```
λ x y . x

      x : 1
λ y . x : 2 -> 1

=> 1 -> 2 -> 1 => A -> B -> A
```

```
         3
        ---
λ x y . x y
        | |
        1 2

1 |-> 2 -> 3

=> (2 -> 3) -> 2 -> 3 => (A -> B) -> A -> B
```

```
λ x . x

x : 1

=> 1 -> 1 => A -> A
```

This is sufficient to give a principal type without justification.

For the second part of the question:

```
PPc(λ x y z . x z (y z)) = (5 -> 6 -> 7) -> (5 -> 6) -> 5 -> 7
          PPc(λ x y . x) = 1 -> 2 -> 1
            PPc(λ x . x) = 1 -> 1
```

We haven't made this safe for unification yet. The 2nd and 3rd term share variables, so we need to rename them.

```
PPc(λ x y z . x z (y z)) = < {}, (5 -> 6 -> 7) -> (5 -> 6) -> 5 -> 7 > = P1
          PPc(λ x y . x) = < {}, 1 -> 2 -> 1 > = P2
            PPc(λ x . x) = < {}, 4 -> 4 > = P3
```

All of the contexts are empty in this case.

```
            This 8 is the representation of applying P1 to P2.
                                   |
1st call to unify: unify P1 (P2 -> 8)
                     = (5 -> 6 -> 7) -> (5 -> 6) -> 5 -> 7     (1 -> 2 -> 1) -> 8
                   unify (5 -> 6 -> 7) (1 -> 2 -> 1)
                     = 5 |-> 1, 6 |-> 2, 7 |-> 1
                   unify (1 -> 2) -> 1 -> 1     8
                     = 8 |-> (1 -> 2) -> 1 -> 1

Therefore PPc(1st 2nd) = < {}, (1 -> 2) -> 1 -> 1 >
```

```
PPc(1st 2nd 3rd) would then be:

unify (1 -> 2) -> 1 -> 1     (4 -> 4) -> 9:
unify (1 -> 2) (4 -> 4)
  = 1 |-> 4, 2 |-> 4
unify (4 -> 4) 9
  = 9 |-> 4 -> 4
```

For that second example:

```
PPc((λ x y . x y) (λ x . x)):

unify (2 -> 3) -> 2 -> 3    (1 -> 1) -> 4
  = 4 |-> 1 -> 1
```

Notice that their principal types are equal.

Let's go back to...

# $\Lambda^N$

Let us define type assignment for the four building blocks for $\Lambda^N$, `(A x)`, `(-> I)`, `(-> E)`. It's mostly the same as plain lambda calculus, but now we have to worry about names in the current environment $\Gamma; \mathcal{E} \vdash M : A$.

E.g. Let's type:

```
I = λ x . x;
I I
```

Well we know that `(λ x . x)` has the same principal type in both `I`s, so we need to use substitution instances to generate types.

$$\begin{align*}
    (Call)&\ \frac{}{\Gamma; \mathcal{E}, \text{name} : A \vdash name : S A} \\
    (\epsilon)&\ \frac{}{\mathcal{E} \vdash \epsilon : \diamond} \\
    (Defs)&\ \frac{\mathcal{E} \vdash \text{Defs} : \diamond \hspace{2em} \emptyset \vdash M : A}{\mathcal{E}, name : A \vdash \text{Defs} : \text{name} = M : \diamond}\\
    (Program)&\ \frac{\mathcal{E} \vdash \text{Defs} : \diamond \hspace{2em} \Gamma; \mathcal{E} \vdash M : A}{\Gamma; \mathcal{E} \vdash \text{Defs} : M : A}
\end{align*}$$

Given:

```
I = λ x . x ;
B = λ x y z . x (y z) ;
K = λ x y . x ;
S = λ x y z . x z (y z) ;
S (B I) (K I)
```

Find a suitable environment for this program, and give a type-derivation for the final term.

```
I = λ x . x
          |
          1

λ x . x : 1 -> 1 === A -> A

                  4
                -----
B = λ x y z . x (y z)
              |  | |
              1  2 3

2 |-> 3 -> 4
1 |-> 4 -> 5

=> (4 -> 5) -> (3 -> 4) -> 3 -> 5 === (B -> C) -> (A -> B) -> A -> C

K = λ x y . x
            |
            1

λ y . x : 2 -> 1
=> 1 -> 2 -> 1 === A -> B -> A


               5    6
              --- -----
S = λ x y z . x z (y z)
              | |  | |
              1 2  3 4

3 |-> 4 -> 6
1 |-> 2 -> 5 -> 6
2 |-> 4

 => (4 -> 6 -> 7) -> (4 -> 6) -> 4 -> 7
=== (A -> B -> C) -> (A -> B) -> A -> C
```

$\mathcal{E} = \{\ I : 1 \to 1; B : (2 \to 3) \to (1 \to 2) \to 1 \to 3; K : 1 \to 2 \to 1; S : (1 \to 2 \to 3) \to (1 \to 2) \to 1 \to 3 = \pi_s\ \}$

$$\dfrac{\emptyset \vdash S (B I) (K I) : (8 \to 7) \to 7 = ((9 \to 9) \to 7) \to 7}{
    \dfrac{\emptyset \vdash S (B I) : ((8 \to 7) \to 8) \to (8 \to 7) \to 7}{
        \emptyset \vdash S : S_0(\pi_s)
        \hspace{2em}
        \dfrac{\emptyset \vdash B I : ((8 \to 7) \to 8) \to (8 \to 7) \to 7}{
            \dfrac{\emptyset \vdash B : (7 \to 7) \to (8 \to 7) \to 8 \to 7}{}
            \hspace{2em}
            \dfrac{\emptyset \vdash I : 7 \to: 7}{}
        }
    }
    \hspace{2em}
    \dfrac{\emptyset \vdash K I : (8 \to 7) \to 7 = ((9 \to 9) \to 7) \to 9 \to 9}{
        \dfrac{\emptyset \vdash K : 8 \to (8 \to 7) \to 8}{}
        \hspace{2em}
        \dfrac{\emptyset \vdash I : 9 \to 9}{}
    }
}$$

Where

$$\begin{align*}
    S_0 = 1 &\mapsto 8 \to 7 \\
    2 &\mapsto 8 \\
    3 &\mapsto 7 \\
    \\
    \text{Finally, this substitution applies to the last type:}\ 8 &\mapsto 9 \to 9
\end{align*}$$

Reducing `S (B I) (K I)` to normal form...

```
    S (BI) (KI)
 -> (λ x y z . x z (y z)) (B I) (K I)
->2 λ z . B I z (K I z)
 -> λ z . (λ a b c . a (b c)) I z (K I z)
->3 λ z . I (z (K I z))
->2 λ z . z (K I z)
->3 λ z . z I
 -> λ z . z (λ d . d)
```

Hence, we have shown that this system supports polymorphism via substitutions.
