# Mycroft's Change

So we know we already have that:
$$\dfrac{
    \Gamma, f : A \vdash E : A
}{
    \Gamma \vdash \text{fix } f . E : A
}$$
Well, why don't we make this polymorphic...?
$$\dfrac{
    \Gamma, f : \sigma \vdash E : \sigma
}{
    \Gamma \vdash \text{fix } f . E : \sigma
}$$
Hmm, typing this is now undecidable, like with $F = \lambda f . F$...

Mycroft came along and said, "what if we just make just $f$ in that expression polymorphic and attempt to resolve it as soon as possible?":
$$\begin{align*}
    F &= \lambda f . F \\
    \text{where } f &: \sigma \mapsto \forall \varphi . \varphi \\
    F &: A
\end{align*}$$
The algorithm is now correct, but semi-decidable. However, we can still use it to make a type-checking system, like:
$$\begin{align*}
    &fun : type\\
    &\left[
        \begin{array}{l}
            \\
            \text{rec } fun : S\ type\\
            \\
        \end{array}
    \right.
\end{align*}$$
We are still trying to solve:
$$\begin{align*}
    \mathcal{W}\ \Gamma\ (\text{fix } g . E) &= \left< S_2 \circ S_1, S_1\ A\right> \\
    \left< S_1, \sigma \right> &= \mathcal{W}\ (\Gamma, g : \mathcal{X})\ E \\
    S_2 &= \text{unify}\ (S_1\ \alpha)\ \sigma \\
    \text{but...}\ &S_1\ \alpha\ \text{is what exactly?}
\end{align*}$$
![[MycTA.png]]

![[MycTC.png]]

# Combinatory Logic

Haskell Curry came up with these following operators:

- $\mathbf{S}\ x\ y\ z \to x\ z\ (y\ z)$.
- $\mathbf{K}\ a\ b \to a$.

These map very nicely into the lambda calculus... but the reverse is also true. But:

- $CL \to \Lambda$: Easy!
- $\Lambda \to CL$: ... Not so easy.

So let our grammar for this logic be:
$$t ::= \mathbf{S}\ |\ \mathbf{K}\ |\ t_1\ t_2$$

E.g. $\lceil S\ t_1\ t_2\ t_3 \rfloor_\Lambda = (\lambda x y z . x z (y z))\ \lceil t_1 \rfloor\ \lceil t_2 \rfloor\ \lceil t_3 \rfloor \to^3 \lceil t_1 \rfloor\ \lceil t_3 \rfloor\ (\lceil t_2 \rfloor\ \lceil t_3 \rfloor)$

$$\begin{align*}
    |\lceil MN \rfloor| &= |\lceil M \rfloor|\ |\lceil N \rfloor| \\
    |\lceil \lambda x . M \rfloor| &= \text{Fun } x\ |\lceil M \rfloor| \\
    \lceil\ |\lceil M \rfloor|\ \rfloor &\to^* M\\
    \\
    \text{Fun } x\ x &= \mathbf{S\ K\ K} = \mathbf{I} \\
    \text{Fun } x\ t &= \mathbf{K}\ t\ (x\ \text{not in } t) \\
    \text{Fun } x\ (t_1\ t_2) &= \mathbf{S}\ (\text{Fun } x\ t_1)\ (\text{Fun } x t_2)
\end{align*}$$

Let us also define:

- $\mathbf{I}\ x \to x$.
- $\mathbf{B}\ x\ y\ z \to x\ (y\ z)$.
- $\mathbf{C}\ x\ y\ z \to x\ z\ y$.

And some optimisation rules:

- $\mathbf{S}\ (\mathbf{K}\ x)\ (\mathbf{K}\ y)\ t_1 \to^* \mathbf{K}\ (x\ y)\ t_1$.
- $\mathbf{S}\ (\mathbf{K}\ x)\ y \to \mathbf{B}\ x\ y$.
- $\mathbf{S}\ x\ (\mathbf{K}\ y) \to \mathbf{C}\ x\ y$.

We can see that if our arguments to $\mathbf{S}$ are of a certain shape, we can do a rewrite. This is the basis of pattern-matching, and we can further extend this if we want.

So what does that mean for us? In $\Lambda^N$, with our $\text{Defs} : \text{Program}$, our combinators are terms where:

$$\begin{align*}
    \dfrac{}{\mathcal{E} \vdash \text{Term} : A} &\\
    \dfrac{}{\mathcal{E} \vdash F : S\ A}\ &(F : A \in \mathcal{E}) \\
    \\
    \mathcal{E} &= \{ \mathbf{S} : (1 \to 2 \to 3) \to (1 \to 2) \to 1 \to 3, \mathbf{K} : 4 \to 5 \to 4 \}
\end{align*}$$

$(\to E)$ remains unchanged, but we have two extra rules:
$$\begin{align*}
    (\mathbf{S})\ &\dfrac{}{\vdash \mathbf{S} : (A \to B \to C) \to (A \to B) \to A \to C} \\
    (\mathbf{K})\ &\dfrac{}{\vdash \mathbf{K} : A \to B \to A}
\end{align*}$$

This system is usually referred to as the Hindley-Milner type assignment system.

# Term Rewriting

In such a **Term Rewriting System**, we have rewrite rules, which are pairs where $\left< lhs, rhs \right>$ encodes a transformation $lhs \to rhs$, where $lhs = F\ t_1, \dots, t_n$, and $F$ is some name, and all variables in the right-hand side all occur in the left-hand side.

We also have reduction rules such that $lhs^R \to rhs^R$. The rewrite rules encode the reduction steps, where $C[lhs^R] \to C[rhs^R]$.

We also have terms defined as: $t, u ::= x\ |\ t\ u\ |\ F$.

So how do we type this, since we don't have any fixed rewrite rules or the escape in the form of $\mathbf{S}$ and $\mathbf{K}$?

We could give terms types like: $\Gamma; \mathcal{E} \vdash t : A$ as usual, then we get the following rules:
$$\begin{align*}
    (A x)\ &\dfrac{}{\Gamma, x : A; \mathcal{E} \vdash x : A} \\
    (F)\ &\dfrac{}{\Gamma; \mathcal{E}, F : A \vdash F : S\ A}\\
    (\to E)\ &\text{is the same as usual.}
\end{align*}$$
We want subject reduction for free, so we need to make a typing rule for $lhs \to rhs$... well, we could say that $\Gamma; \mathcal{E} \vdash lhs : A$ and $\Gamma; \mathcal{E} \vdash rhs : A$.

Any defined symbol or rule $(F)$ has type $\mathcal{E}\ F$.

So do we get type assignment? Not yet. Our $lhs \to rhs$ rule is not quite correct.

# $\lambda \mathbf{x}$: Lambda Calculus as a Term-Rewriting System

First, is $(\lambda x . M) N \to M [N / x]$... no. The substitution is implicit, unlike in a TRS where the rewrites are explicit. So we need $(\lambda x . M) N \to M \left< x := N \right>$.

So now our lambda calculus grammar is now: $M, N ::= x\ |\ \lambda x . M\ |\ MN\ |\ M \left< x := N \right>$, and with it:

- $(\lambda x . M) N \to M \left< x := N \right>$... which becomes $Appl\ (Abst\ (Var\ x)\ M)\ N \to Subst\ M\ x\ N$.
- $(M N) \left< x := L \right> \to M \left< x := L \right> N \left< x := L \right>$... which becomes $Subst\ (Appl M N)\ X\ L \to Appl\ (Subst\ M\ x\ L)\ (Subst\ N\ x\ L)$.
- $(\lambda y . M) \left< x := L \right> \to \lambda y . M \left< x := L \right>$... which becomes $Subst\ (Abst\ y\ M)\ x\ L \to Abst\ y\ (Subst\ M\ x\ L)$.
- $x \left< x := L \right> \to L$... which becomes $Subst\ x\ x\ L \to L$.
- $y \left< x := L \right> \to y \hspace{1em} (x \neq y)$... which becomes $Subst\ y\ x\ L \to y$, still given that $x \neq y$.

Which is now a TRS.
