So our rules define the following to derive types:

$$\frac{}{\Gamma, x : A \vdash x : A}\ (A\ x)$$
$$\frac{\Gamma, x : A \vdash M : B}{\Gamma \vdash \lambda x . M : A \to B}\ (\to I)$$
$$\frac{\Gamma \vdash M : A \to B \hspace{2em} \Gamma \vdash N : A}{\Gamma \vdash M N : B}\ (\to E)$$

... but these rules don't actually tell us what `A` and `B` actually are.

What if we want to say:
- Give a type to `x` given: $\vdash x$? Simple enough, just take any type: $x : A \vdash x : A$.
- Give a type to an abstraction, $\lambda x . M$?
	- If $x \in \Gamma$, then we have our `(-> I)` rule.
	- Otherwise, if $x \notin \Gamma$, then we can assume $x \notin M$, so we can give `x` any type.
- Give a type to an application, $M N$.
	- Well, if our `M` and `N` are assigned types from different $\Gamma$s, we need to take the union of both $\Gamma$s... while being careful about type conflicts between types.

Well, we will find an algorithm that assigns principal pairs. This algorithm, `PPc`, will run on some expression `M` and give us a pair of $\left< \Pi, P\right>$ (a context and a type):
- Then $\Pi \vdash M : P$.
- If $\Gamma \vdash M : A \land \left< \Pi, P \right>$: there exists a substitution $S$ such that $S\Pi = \Gamma$, $SP = A$.

It will peform the most generic type assignment with the least amount of arrow types possible.

Substitutions will substitute type variables with some generic type. This is the basis for the algorithm. It is inductively defined as:

$$\begin{align*}
S\ :\ &(\varphi \mapsto C)\ \varphi &&= C \\
&(\varphi \mapsto C)\ \varphi' &&= \varphi'\ (\varphi \neq \varphi') \\
&(\varphi \mapsto C)\ A \to B &&= ((\varphi \mapsto C)\ A) \to ((\varphi \mapsto C)\ B)
\end{align*}$$

This principle is the same as unification (see also Prolog's unification). It tries to find things that match:

```
unify A B tries to find S such that SA = SB
```

- unify $\varphi\ C = (\varphi \mapsto C), \varphi \neq C$
- unify $\varphi\ \varphi = \text{id}$
- unify $C\ \varphi =$ unify $\varphi\ C$
- unify $(A \to B)\ (C \to D) = S_2 \circ S_1$ where $S_1 =$ unify $A$ $C$, and $S_2 =$ unify $(S_1 B)$ $(S_1 D)$

![[UnifyContexts.png]]

Unification is incomplete; it can fail. This means there is a type error somewhere. So:
- $PPc\ X = \left< x : \varphi; \varphi \right>$
- $PPc\ \lambda x . M = \left< \Pi, P \right>$, where:
	- $\left< \Pi', P' \right> = PPc\ M$ if $x : A \in \Pi'$
	- $\Pi = \Pi' \setminus x : A$ if $x \in P_v(M)$
	- $P = A \to P'$ if $x \in P_v(M)$
	- $\Pi = \Pi'$ if $x \notin P_v(M)$
	- $P = UNDEF \to P'$ if $x \notin P_v(M)$

Given:
- $\left< \Pi_1; P_1 \right> \Rightarrow \Pi_1 \vdash M : P_1$
- $\left< \Pi_2; P_2 \right> \Rightarrow \Pi_2 \vdash N : P_2$

And we want $P_1 = A \to B$... we unify:
- Case 1: unify $A\ P_2 = S$, which gives $P = SB$.
- Case 2: $P_1 = \varphi \sim P_2 \to \varphi''$, where:
	- $S = \varphi \mapsto P_2 \to \varphi''$
	- $P = \varphi''$

So:

$PPc\ MN = \left< \Pi; P \right>$:
- $\left< \Pi_1, P_1 \right> = PPc\ M$
- $\left< \Pi_2, P_2 \right> = PPc\ N$
- $S = \text{unify}\ P_1\ (P_2 \to \varphi)$
- $S' = \text{unifyC}\ (S \Pi_1)\ (S \Pi_2)$ (Context unification)
- $\Pi = S' \circ S\ (\Pi_1 \circ \Pi_2)$
- $P = S' \circ S\ \varphi$

This algorithm fails if unification fails (when there's a type mismatch, etc.).

To show the 2nd property of $PPc$, we need a lemma that says if $\Gamma \vdash M : A$, then $S \Gamma \vdash M : S A$.

In order to make this more efficient (e.g. to type the identity function applied to itself, we need to extend lambda calculus with names).

# $\Lambda^N$: Named Lambda Calculus

This lambda calculus extension allows the defining of names for closed lambda terms (terms that have no free variables in them).

- $M, N ::= x\ |\ \lambda x . M\ |\ M N\ |\ \text{name}$
- $\text{name} ::=$ any string of characters
- $\text{Defs} ::= \text{Defs}; \text{name} = M\ |\ \epsilon$ ($M$ is closed, and does not have $\text{name}$s in them.)
- $\text{Program} ::= \text{Defs} : M$ ($M$ is allowed names and free variables here.)

So how do we run a program?

$$\frac{}{(\lambda x . M) N \to M [N / x]}$$
$$\frac{}{\text{name} \to M}\ (\text{name} = M \in \text{Defs})$$
$$\frac{M \to^{*} N}{\text{Defs} : M \to^{*} \text{Defs} : N}$$

There are also the normal contextual rules and transitive closure rules.

![[LambdaN.png]]

It is also possible to convert $\Lambda^N$ to $\Lambda$ by simply substituting all names with their respective expressions from $\text{Defs}$ (and in the case of a program, removing $\text{Defs}$ too).
