### Exercise 4.8:

```
E = λ x y . x y
      | |   --- 3
      1 2

1 |- 2 -> 3

=> E : (2 -> 3) -> 2 -> 3
```

```
              --------- 6
S = λ x y z . x z (y z)
      | | | 4 --- ----- 5
      1 2 3

2 |- 4 -> 5
1 |- 3 -> 5 -> 6

=> S : (3 -> 5 -> 6) -> (3 -> 5) -> 3 -> 6
```

```
(E E) : unify ((1 -> 2) -> 1 -> 2) (((3 -> 4) -> 3 -> 4) -> 5)

5 |-> 1 -> 2
1 |-> 3 -> 4
2 |-> 3 -> 4

=> (E E) : (3 -> 4) -> 3 -> 4
```

```
S (E E) : unify (5 -> 6 -> 7) ((3 -> 4) -> 3 -> 4)

7 |-> 3 -> 4
6 |-> 3
5 |-> 3 -> 4

=> S (E E) : ((3 -> 4) -> 3) -> (3 -> 4) -> 4
```

Skipping over the derivation for `rec Y`, which will require the `pp` algorithm, and using the known result of `Y : (10 -> 10) -> 10`.

```
Y (S (E E)) : unify ((10 -> 10) -> 10) (((3 -> 4) -> 3) -> (3 -> 4) -> 4)

-- TODO.
```

# Milner's $\mathbf{ML}$

ML, short for "Meta Language", was a formal type discipline presented for polymorphic procedures in a simple programming language called $\mathcal{L}_\mathbf{ML}$, designed to express that certain procedures work well on objects of a wide variety. This kind of procedure is called *(shallow) polymorphic*, and it is essential to obtain enough flexibility in programming.

Like many other systems, $\mathcal{L}_\mathbf{ML}$ is based on the Lambda Calculus, although we have left the scope of a "true" lambda calculus.

![[MLTAS.png]]

![[MLT.png]]

![[MTA.png]]

(In other words, for $\forall I$, $\varphi \notin \Gamma$.)

Let's type:

$$\dfrac{
    \vdash \text{let i = } \lambda x . x \text{ in } \text{ii} : A \to A 
}{
    \dfrac{
        \vdash \lambda x . x : \forall \varphi . \varphi \to \varphi
    }{
        \dfrac{
            \vdash \lambda x . x : \varphi \to \varphi
        }{
            \dfrac{
                x : \varphi \vdash x : \varphi
            }{
            } (A x)
        } (\to I)
    } (\forall I)
    \hspace{2em}
    \dfrac{
        \text{i} : \forall \varphi . \varphi \to \varphi\vdash \text{ii} : A \to A
    }{
        \dfrac{
            \text{i} : \forall \varphi . \varphi \to \varphi \vdash \text{i} : (A \to A) \to A \to A
        }{
            \dfrac{
                \text{i} : \forall \varphi . \varphi \to \varphi \vdash \text{i} : \forall \varphi . \varphi \to \varphi
            }{} (A x)
        } (\forall E)
        \hspace{2em}
        \dfrac{
            \text{i} : \forall \varphi . \varphi \to \varphi \vdash \text{i} : A \to A
        }{
            \dfrac{
                \text{i} : \forall \varphi . \varphi \to \varphi \vdash \text{i} : \forall \varphi . \varphi \to \varphi
            }{} (A x)
        } (\forall E)
    } (\to E)
} (\text{let})$$
