For reference to the **S K I** terms, see [[TS_2022-10-10]].

Exercise 1.29:

```
(λ x y z . x z (y z)) (λ a b . a) = S K
-> λ y z . (λ a b . a) z (y z)
-> λ y z . (λ b . z) (y z)
-> λ y z . z
=> Has normal form (... and HNF)

(λ f . (λ x . f (x x)) (λ x . f (x x))) (λ a . a) = Y I
.. (λ a . a) is renamed as I for short
-> (λ x . I (x x)) (λ x . I (x x))
-> I ((λ x . I (x x)) (λ x . I (x x)))
-> (λ x . I (x x)) (λ x . I (x x))
-> (λ x . x x) (λ x . x x)
=> does not normalise, nor have a HNF

(λ f . (λ x . f (x x)) (λ x . f (x x))) (λ a b . a) = Y K
-> (λ x . (λ a b . a) (x x)) (λ x . (λ a b . a) (x x))
-> (λ a b . a) ((λ x . (λ a b . a) (x x)) (λ x . (λ a b . a) (x x)))
-> λ b . ((λ x . (λ a b . a) (x x)) (λ x . (λ a b . a) (x x)))
->2 λ b . (λ x b . x x) (λ x b . x x)
=> does not normalise, nor have a HNF
(correct this one please)

(λ f . (λ x . f (x x)) (λ x . f (x x))) (λ a b . b)
-> (λ x . (λ a b . b) (x x)) (λ x . (λ a b . b) (x x))
->2 (λ x b . b) (λ x b . b)
-> λ b . b
=> Has normal form (... and HNF)

(λ f . (λ x . f (x x)) (λ x . f (x x))) (λ a b . a b)
-> (λ x . (λ a b . a b) (x x)) (λ x . (λ a b . a b) (x x))
->2 (λ x b . (x x) b) (λ x b . (x x) b)
-> λ b . ((λ x b . (x x) b) (λ x b . (x x) b)) b
=> repeats... does not normalise, nor have a HNF
```

Lambda calculus, studied by its semantics, is a rising research topic.

# Type Assignment

Let's do an input-output analysis.

```
λ x . M : A -> B
  |   |
  A   B

     M N -> R
     | |    |
A -> B A    B
```

```
A |- B
--------- (If assuming A gives you B, you get A -> B.)
|- A -> B
```

We need types, like (`A -> B`). Let's define a grammar.

```
   Type variable
         |
A, B ::= γ | A -> B
```

Let's try to assign some types:

```
Γ |- M : A -> B     N : A
------------------------- (-> E)
       Γ |- M N : B
```

Therefore:

```
Γ, x : A   |-   M : B
--------------------- (-> I)
Γ |- λ x . M : A -> B
```

Γ is an unordered list of type assignments, a **context** of the expression, that acts as a function assigning types to term variables.

```
----------------- (A x) "Action" / "Axiom"
Γ, x : a |- x : A

"Assuming x is of type A in context Γ, x is of type A."

(Bound variables give constraints for types within a context.)
```

```
Γ |- M : A ≜ there exists a derivation built out of (A x), (-> I), (-> E) that has this at the bottom
```

Let's type `λ x . x`, `λ a b . a b`, `λ a b . a`.

```
--------------------- (A x)
Γ, x : A   |-   x : A
--------------------- (-> I)
Γ |- λ x . x : A -> A

------------------------------- (A x)  -------------------------- (A x)
a : A -> B, b : A |- a : A -> B        a : A -> B, b : A |- b : A
----------------------------------------------------------------- (-> E)
   a : A -> B, b : A |- a b : B
----------------------------------- (-> I)
 a : A -> B |- λ b . a b : A -> B
----------------------------------- (-> I)
|- λ a b . a b : (A -> B) -> A -> B

Deriv[K]
----------------------
  Γ, a : A |- a : A
---------------------- (A x)
Γ, a: A, b : B |- a: A
------------------------------------------------- (-> I)
          Γ, a : A |- λ b . a : B -> A
------------------------------------------------- (-> I)
          Γ |- λ a b . a : A -> B -> A

(Context can be omitted if no free variables exist in the expression.)
```

Exercise 2.17:

***PROTIP: YOU ARE ALLOWED TO DO THESE TREES UPSIDE DOWN!***

```
Deriv[S]
------------------          --------           -------------       --------
|- x : A -> B -> C          |- z : A           |- y : A -> B       |- z : A
------------------ (A x)    ----------- (A x)  ------------- (A x) ------------ (A x)
        |- x : A -> B -> C, z : A                  |- y : A -> B, z : A
        ------------------------------- (-> E)     --------------------------- (-> E)
                                |- x z : (B -> C), y z : B
                                ---------------------------- (-> E)
x : A -> B -> C, y : A -> B, z : A |- x z (y z) : C
------------------------------------------------------------ (-> I)
x : A -> B -> C, y : A -> B |- λ z . x z (y z) : A -> C
------------------------------------------------------------ (-> I)
x : A -> B -> C |- λ y z . x z (y z) : (A -> B) -> A -> C
------------------------------------------------------------ (-> I)
|- λ x y z . x y (y z) : (A -> B -> C) -> (A -> B) -> A -> C
```

```
|- b : A          |- c : B
-------- (A x)    -------- (A x)
   b : A, c : B |- c : B
-------------------------- (-> I)
b : A |- λ c . c -> B -> B
-------------------------- (-> I)
|- λ b c . c : A -> B -> B
```

```
(λ a b c . a c (b c)) (λ x y . x) : (B -> A) -> B -> B

This is S K, which:

(λ a b c . a c (b c)) : (A -> B -> C) -> (A -> B) -> A -> C from Deriv[S] (above)
(λ x y . x) : A -> B -> A from Deriv[K] (above)

therefore, substituting some letters:

S K = (A -> B) -> A -> A ... and since types are universally quantified, is identical to (B -> A) -> B -> B
```

***REMINDER: UPSIDE DOWN TREES ARE OKAY!***
