Exercise 2.17:

```
 λ b c . c : A -> B -> B
------------------------- (-> I)
b : A |- λ c . c : B -> B
------------------------- (-> I)
  b : A, c : B |- c : B
-------- (A x)   -------- (A x)
|- b : A         |- c : B
```

```
Rewrite (λ x y . x) c (b c) as ((λ x . (λ y . x)) c) (b c).

   λ b c . ((λ x . (λ y . x)) c) (b c) : (B -> A) -> B -> B
-------------------------------------------------------------- (-> I)
   b : B -> A |- λ c . ((λ x . (λ y . x)) c) (b c) : B -> B
-------------------------------------------------------------- (-> I)
     b : B -> A, c : B |- ((λ x . (λ y . x)) c) (b c) : B
-------------------------------------------------------------- (-> E)
|- (λ x . (λ y . x)) c : A -> B,                      b c : A
--------------------------------------------- (-> E)  ------------- (-> E)
|- λ x . (λ y . x) : B -> A -> B,       c : B         |- b : B -> A, c : B
-------------------------------- (-> I) ----- (A x)   -------- (A x) -----
 x : B |- λ y . x : A -> B
--------------------------- (-> I)
x : B,       y : A |- x : B
----- (A x)  ----- (A x)
```

# Subject Reduction

If `Γ |- M : A` and `M ->* N` implies `Γ |- N : A`. Note that subject expansion (the reverse), does not work.

So how do we prove it?

Well, it is an if statement, so we can probably find a derivation that leads up to this conclusion. We can do this by induction on the three rules for type derivation `(A x)`, `(-> I)` and `(-> E)`.

Here is an incomplete version:

If `Γ |- M : A` and `M ->* N` then `Γ |- N : A`.

By induction on the definition of reduction, we have seven cases:

Single-Step Reduction
1. `M = (λ x . P) Q => N = P [Q / x]`
	- If `M = (λ x . P) Q`, then by `(-> E)` there exists `B` such that `Γ |- λ x . P : B -> A` and `Γ |- Q : B`. Then by `(-> I)`, `Γ, x : B |- P : A`. By lemma (substitution) `Γ |- P [Q / x] : A`.
2. `P -> P' => λ x . P -> λ x . P'`
	-  If `M = λ x . P` and `P -> P'`, then by `(-> I)`, `A = B -> C` and `Γ, x : B |- P : C`. By induction, `Γ, x : B |- P' : C`. So by `(-> I)`, we can get `Γ |- λ x . P' : B -> C`, so `Γ |- λ x . P' : A`.
3. `P -> P' => P R -> P' R`
	- If `M = P R` and `P -> P'`, then by `(-> E)` there exists a term `B` such that `Γ |- P : B -> A` and `Γ |- R : B`. By induction, `Γ |- P' : B -> A`. So by `(-> E)` we have `Γ |- P' R : A`.
4. `P -> P' => R P -> R P'`
	- If `M = R P` and `P -> P'`, then by `(-> E)` there exists some term `B` such that `Γ |- P : A` and `Γ |- R : A -> B`. By induction, `Γ |- P' : A`. So by `(-> E)` we have `Γ |- R P' : B`. 

Multi-Step Reduction
5. `P -> P' => P ->* P'`
	- If we have `P -> P'`, then trivially we have `P ->* P'` from the definition of `->*`. (**???**)
6. `P ->* R & R ->* S => P ->* S`
7. `P ->* P`

**Substitution Lemma**: For all `Γ`, `x`, `A`, `B`, `P` and `Q`, if `Γ, x : B |- P : A` and `Γ |- Q : B` then `Γ |- P [Q / x] : A`... so `(λ y . R) [Q / x] = λ y . R [Q / x]`.

By induction over the definition of term substitution:

1. `P = x`: then `Γ, x : B |- x : A`, so `A = B`. So `Γ |- Q : A`, and `x [Q / x] = Q`.
2. `P = y` and `y != x`: then `Γ, x : B |- y : A`, so `Γ = Γ', y : A`. By `(A x)`, `Γ |- y : A` and `y [Q / x] = y`.
3. `P = λ y . R`: Then `Γ, x : B |- λ y . R : A`. So `A = C -> D`. Then by `(-> I)`, `Γ, x |- B, y : C |- R : D`. By induction (i.e. "we can assume ... and by that assumption ... holds"), `Γ, y : C |- R [Q / x] : D`, so by `(-> I)`, `Γ |- λ y . R [Q / x] : C -> D`, so `Γ |- (λ y . R) [Q / x] : A`.

**Induction**: for all `R`, if `R ->* Q`, then `P(R)` implies `P(Q)` for some property `P`.

The principle of induction is that if we have an inductively-defined set V, we have defined the following:

1. `a1, ..., an` in `V` (base cases)
2. if `b1, ..., bm` in `V`, then `f` in `V` (inductive cases)

`(*)` If another set `W` satisfies `1.` and `2.`, then `V` is a subset, or is equal to `W`.

A famous example is Peano's Axioms for natural numbers:

1. 0 is in `N`
2. if `n` in `N` then `S(n)` in `N`

We have a base case, `0`, and a constructor case. In this case, this is structural induction, as we are adding structure to the constructed objects. If `W` satisfies `1.` and `2.`, then `N` is a subset, or is equal to `W`.

In particular, `W` is the subset of natural numbers that satisfy some predicate `P`. If `W` is a subset or is equal to `N`, this means that the predicate `P` holds for all `N`. To prove this, we need to show:

3. `0` is in `W`
4. if `n` in `W`, then `n + 1` in `W`, that is, if `P(n)` holds, then `P(n + 1)` holds as well

The issue is that numeric / mathematical induction is only one such inductively-defined set. There are **infinitely many** other inductively-defined sets.

Grammars are also inductively defined grammars. Take the lambda calculus definition: `M, N ::= x | (λ x . M) | (M N)`. It is basically an alternate way of writing:

- `x` in `Λ`
- if `M` in `Λ`, then `(λ x . M)` in `Λ`
- if `M, N` in `Λ`, then `(M N)` in `Λ`

Hence this is also an inductively defined set, and we can reason about properties of this set with induction. For example, beta-reduction (single-step).

```
STANDARD DEFINITION

(λ x . M) N -> M [N / x]
P -> Q => | λ x . P -> λ x . Q
          | P M     -> Q M
          | M P     -> Q M
```

This means that the beta-reduction rules are a subset of pairs of lambda terms, `Vβ = ->β` is a subset, or is equal to `Λ²`:

```
SET DEFINITION

1. <(λ x . M) N, M [N / x]> in Vβ
2. if <P, Q> in Vβ then <λ x . P, λ x . Q> in Vβ
                    and <P M, Q M> in Vβ
                    and <M P, M Q> in Vβ
```

We can prove properties of this using induction:

For all `p` in `Vβ` where `P(p)`:
- show that `P(<P M, Q M>)` holds, assuming that `P(P, Q)`.

Another different way of writing this is using inference rules:

```
INFERENCE DEFINITION

------------------------- (β)
(λ x . M) N ->β M [N / x]

      P ->β Q
------------------- (Abst)
λ x . P ->β λ x . Q

  P ->β Q
----------- (AppR)
P M ->β Q M

  P ->β Q
----------- (AppL)
M P ->β M Q
```

You can see the parallels with the `1.`, `2.` definition above, enhanced with some `if-then` information in a succinct way.

Each different writing style gives a different representation of the set in question:
- The first is a lot more syntactic.
- The second reasons more around sets.
- The third provides a framework for reasoning around the objects.

For example, with those inference rules, we can write:

```
          (λ x . x) (λ y . y) ->β λ x . x
-----------------------------------------------------
    λ z . (λ x . x) (λ y . y) ->β λ z . (λ x . x)
-----------------------------------------------------
(λ z . (λ x . x) (λ y . y)) M ->β (λ z . (λ x . x)) M
```

To reason around reduction. But to prove a property for the set, we can pick any of the three definitions above, and use it to prove that *for all `<R, Q> in Vβ`, if `P(<R, Q>)` holds, then*:

- Prove for case (β).
- Prove for case (Abst).
- Prove for case (AppR): show `P(<R M, Q M>)` because `P(<R, Q>)` holds.
- Prove for case (AppL) is symmetric to the proof for case (AppR): show `P(<M R, M Q>)` because `P(<R, Q>)` holds.

Let's look at type assignment and its definitions:

```
SET

1. <Γ, x : A; x; A> in Derivable Statements (DS)
2. if <Γ, x : A; M; B> in DS, then <Γ; λ x . M; A -> B> in DS
   if <Γ; M; A -> B> in DS and <Γ; N; A> in DS then <Γ; M N; B> in DS
```

So if we want to prove some property on this, we have three cases. In inference form, using a `|-` to say that we can derive RHS from LHS (hence the statement is in `DS`), we can say:

```
INFERENCE (<Γ; M; A> in DS ≜ Γ |- M : A (with some derivation above it))

----------------- (A x)
Γ, x : A |- x : A

  Γ, x : A |- M : B
--------------------- (-> I)
Γ |- λ x . M : A -> B

Γ |- M : A -> B    Γ |- N : A
------------------------------ (-> E)
        Γ |- M N : B
```

As before, to prove some property, we still have three cases, with one of these being a terminating / base case.

For all $\Gamma_0, P_0, G_0, A_0$, if $\Gamma \vdash P_0 : A_0$ and $P_0 \to^{*}_{\beta} Q_0$ then $\Gamma_0 \vdash Q_0 : A_0$. We want to show this lemma (the Subject Reduction Lemma, SRL). By induction on the definition of reduction (note that the proof is for typeability, as in, if we can give a type to one thing, from that, we can get the type for the other thing):

- (AppR): Prove `PM -> QM` holds because `P -> Q` holds (alt. wording: Assume `P -> Q`, then to show `PM -> QM`...). If $\Gamma \vdash P M : A$, then by `(-> E)` there exists B such that $\Gamma \vdash P : B \to A$ and $\Gamma \vdash M : B$. SRL holds for $P \to Q$ by induction (assumption; this is the IH). So it also holds for $\Gamma_0 = \Gamma$, $A_0 = B \to A$ (a.k.a. **by induction**). So $\Gamma \vdash Q : B \to A$, and by `(-> E)`, $\Gamma \vdash Q M : A$.
- (AppL): Similar to (AppR) proof, with `M`, `Q` and `R` mirrored respectively.
- (Abst): Prove `λ x . P -> λ x . Q` holds because `P -> Q` holds. Assume $\Gamma \vdash \lambda x . P : A$. Then $\Gamma, x : B \vdash P : C$ and $A = B \to C$. By induction, we can now assume $\Gamma, x : B \vdash Q : C$. Then by `(-> I)`, $\Gamma \vdash \lambda x . Q : B \to C$.
- $(\beta)$: Then $P_0 = (\lambda x . M) N$, $Q_0 = M [N / x]$. Let $\Gamma \vdash (\lambda x . M) N : A$, then by `(-> E)`, there exists some $B$ such that $\Gamma \vdash \lambda x . M : B \to A$ and $\Gamma \vdash N : B$. By `(-> I)` also $\Gamma, x : B \vdash M : A$. By SL (proof below), $\Gamma \vdash M [N / x] : A$.

We have some new inference rules for $\to_{\beta}^{*}$:

$$\frac{M \to_{\beta} N}{M \to_{\beta}^{*} N} \hspace{5em} \frac{M \to_{\beta}^{*} N \hspace{1em} N \to_{\beta}^{*} P}{M \to_{\beta}^{*} P} \hspace{5em} \frac{}{M \to_{\beta}^{*} M} $$

For all $\Gamma_0, M_0, N_0, X_0, A_0, B_0$, if $\Gamma_0, x_0 : B_0 \vdash M_0 : A_0$ and $\Gamma_0 \vdash N_0 : B_0$ then $\Gamma_0 \vdash M_0 [N_0 / x_0] : A_0$. To prove the Substitution Lemma (SL), by induction over the structure of term substitution:

- $M_0 = x$). Let $\Gamma, x_0 : B \vdash x_0 : A$ and $\Gamma \vdash N : B$. Then by `(A x)`, $A = B$, so $\Gamma \vdash N : A$ and $X_0 [N / x_0] \triangleq N$.
- $M_0 = y \neq x$). Let $\Gamma, x_0 : B \vdash y : A$, then by `(A x)`, $y : A \in \Gamma$, so by `(A x)`, $\Gamma \vdash y : A$, and $y [N / x_0] \triangleq y$.
- $M_0 = \lambda x. M'$). Let $\Gamma, x_0 : B \vdash \lambda y. M' : A$, then by `(-> I)`, $A = C \to D$, and $\Gamma, x_0 : B, y : C \vdash M : D$. (To show $\Gamma, y : C \vdash M' [N_0 / x] : D$, so by `(-> I)`...) By induction, we can assume $\Gamma, y : C \vdash M' [N / x_0] : D$; apply `(-> I)`, $\Gamma \vdash \lambda y . M' [N / x_0] : C \to D$, and by $\lambda y . M' [N / x_0] \triangleq (\lambda y . M') [N / x_0]$.
- $M_0 = PQ$). Let $\Gamma \vdash P Q : A$, then by `(-> E)`, there exists some $C$ such that $\Gamma \vdash P : C \to A$ and $\Gamma \vdash Q : C$. By induction, $\Gamma \vdash P [N / x_0] : C \to A$ and $\Gamma \vdash Q [N / x_0] : C$, so by `(-> E)`, $\Gamma \vdash P [N / x_0] Q [N / x_0] : A$, therefore $P [N / x_0] Q [N / x_0] = (P Q) [N / x_0]$.

This lemma says that you can replace a term of some type with another term with the same type without damaging the type derivation / inference.
